src/compiler/meta/OCL_compiler_parser_init.thy
@@ -62,6 +62,7 @@ definition "co10 f g x1 x2 x3 x4 x5 x6 x7 x8 x9 x10 = f (g x1 x2 x3 x4 x5 x6 x7 
 definition "co11 f g x1 x2 x3 x4 x5 x6 x7 x8 x9 x10 x11 = f (g x1 x2 x3 x4 x5 x6 x7 x8 x9 x10 x11)"
 definition "co12 f g x1 x2 x3 x4 x5 x6 x7 x8 x9 x10 x11 x12 = f (g x1 x2 x3 x4 x5 x6 x7 x8 x9 x10 x11 x12)"
 definition "co13 f g x1 x2 x3 x4 x5 x6 x7 x8 x9 x10 x11 x12 x13 = f (g x1 x2 x3 x4 x5 x6 x7 x8 x9 x10 x11 x12 x13)"
+definition "co14 f g x1 x2 x3 x4 x5 x6 x7 x8 x9 x10 x11 x12 x13 x14 = f (g x1 x2 x3 x4 x5 x6 x7 x8 x9 x10 x11 x12 x13 x14)"
 
 definition "ap1 a v0 f1 v1 = a v0 [f1 v1]"
 definition "ap2 a v0 f1 f2 v1 v2 = a v0 [f1 v1, f2 v2]"
@@ -76,6 +77,7 @@ definition "ap10 a v0 f1 f2 f3 f4 f5 f6 f7 f8 f9 f10 v1 v2 v3 v4 v5 v6 v7 v8 v9 
 definition "ap11 a v0 f1 f2 f3 f4 f5 f6 f7 f8 f9 f10 f11 v1 v2 v3 v4 v5 v6 v7 v8 v9 v10 v11 = a v0 [f1 v1, f2 v2, f3 v3, f4 v4, f5 v5, f6 v6, f7 v7, f8 v8, f9 v9, f10 v10, f11 v11]"
 definition "ap12 a v0 f1 f2 f3 f4 f5 f6 f7 f8 f9 f10 f11 f12 v1 v2 v3 v4 v5 v6 v7 v8 v9 v10 v11 v12 = a v0 [f1 v1, f2 v2, f3 v3, f4 v4, f5 v5, f6 v6, f7 v7, f8 v8, f9 v9, f10 v10, f11 v11, f12 v12]"
 definition "ap13 a v0 f1 f2 f3 f4 f5 f6 f7 f8 f9 f10 f11 f12 f13 v1 v2 v3 v4 v5 v6 v7 v8 v9 v10 v11 v12 v13 = a v0 [f1 v1, f2 v2, f3 v3, f4 v4, f5 v5, f6 v6, f7 v7, f8 v8, f9 v9, f10 v10, f11 v11, f12 v12, f13 v13]"
+definition "ap14 a v0 f1 f2 f3 f4 f5 f6 f7 f8 f9 f10 f11 f12 f13 f14 v1 v2 v3 v4 v5 v6 v7 v8 v9 v10 v11 v12 v13 v14 = a v0 [f1 v1, f2 v2, f3 v3, f4 v4, f5 v5, f6 v6, f7 v7, f8 v8, f9 v9, f10 v10, f11 v11, f12 v12, f13 v13, f14 v14]"
 
 definition "ar1 a v0 z = a v0 [z]"
 definition "ar2 a v0 f1 v1 z = a v0 [f1 v1, z]"
@@ -90,6 +92,7 @@ definition "ar10 a v0 f1 f2 f3 f4 f5 f6 f7 f8 f9 v1 v2 v3 v4 v5 v6 v7 v8 v9 z = 
 definition "ar11 a v0 f1 f2 f3 f4 f5 f6 f7 f8 f9 f10 v1 v2 v3 v4 v5 v6 v7 v8 v9 v10 z = a v0 [f1 v1, f2 v2, f3 v3, f4 v4, f5 v5, f6 v6, f7 v7, f8 v8, f9 v9, f10 v10, z]"
 definition "ar12 a v0 f1 f2 f3 f4 f5 f6 f7 f8 f9 f10 f11 v1 v2 v3 v4 v5 v6 v7 v8 v9 v10 v11 z = a v0 [f1 v1, f2 v2, f3 v3, f4 v4, f5 v5, f6 v6, f7 v7, f8 v8, f9 v9, f10 v10, f11 v11, z]"
 definition "ar13 a v0 f1 f2 f3 f4 f5 f6 f7 f8 f9 f10 f11 f12 v1 v2 v3 v4 v5 v6 v7 v8 v9 v10 v11 v12 z = a v0 [f1 v1, f2 v2, f3 v3, f4 v4, f5 v5, f6 v6, f7 v7, f8 v8, f9 v9, f10 v10, f11 v11, f12 v12, z]"
+definition "ar14 a v0 f1 f2 f3 f4 f5 f6 f7 f8 f9 f10 f11 f12 f13 v1 v2 v3 v4 v5 v6 v7 v8 v9 v10 v11 v12 v13 z = a v0 [f1 v1, f2 v2, f3 v3, f4 v4, f5 v5, f6 v6, f7 v7, f8 v8, f9 v9, f10 v10, f11 v11, f12 v12, f13 v13, z]"
 
 subsection{* i of ... *} (* i_of *)
 
